Port CR proof.

challenge_response.v
@@ -25,117 +25,24 @@ Notation iProp := (iProp Σ).
 
 Implicit Types t : term.
 Implicit Types s : session_view.
-Implicit Types l : level.
 Implicit Types rl : role.
 
 Class crG := {
   in_cr_sessG :> sessionG Σ;
-  in_cr_honestG :> inG Σ (authR (prodUR (gsetUR term) (gsetUR term)));
   cr_sess_name : gname;
-  cr_honest_name : gname;
 }.
 
 Context `{!crG}.
-
-Global Instance cr_honest_authG : authG Σ (prodUR (gsetUR term) (gsetUR term)).
-Proof. constructor; apply _. Qed.
-
-Definition cr_honest_proj rl : gset term * gset term → gset term :=
-  if rl is Init then fst else snd.
-
-Definition cr_res_of_key rl k : gset term * gset term :=
-  if rl is Init then ({[k]}, ∅) else (∅, {[k]}).
-
-Lemma cr_res_of_key_included rl k Ks :
-  cr_res_of_key rl k ≼ Ks ↔
-  k ∈ cr_honest_proj rl Ks.
-Proof.
-case: rl Ks=> [] [K1 K2] /=;
-rewrite pair_included !gset_included;
-split; intuition set_solver.
-Qed.
-
-Definition cr_key rl (k : term) : iProp :=
-  auth_own cr_honest_name (cr_res_of_key rl k).
-
-Global Instance cr_key_persistent rl k : Persistent (cr_key rl k).
-Proof. case: rl; apply _. Qed.
 
 Definition msg2_pred kB t : iProp :=
   ∃ nA nB kA,
     ⌜t = Spec.of_list [nA; nB; TKey Dec kA]⌝ ∧
     session cr_sess_name Resp kA kB nA nB.
 
-Global Instance msg2_pred_persistent kB t :
-  Persistent (msg2_pred kB t).
-Proof. by apply _. Qed.
-
-Lemma msg2_pred_elimG `{Decision G} (ts : list term) kA kB nA nB :
-  ts !! 0 = Some nA →
-  ts !! 1 = Some nB →
-  ts !! 2 = Some (TKey Dec kA) →
-  guarded G (msg2_pred kB (Spec.of_list ts)) -∗
-  guarded G (session cr_sess_name Resp kA kB nA nB).
-Proof.
-iIntros (ts_0 ts_1 ts_2) "tsP".
-rewrite /guarded; case: decide => //= _.
-iDestruct "tsP" as (nA' nB' kA') "[%e #sess]".
-by move/Spec.of_list_inj: e ts_0 ts_1 ts_2 => -> [] -> [] -> [] ->.
-Qed.
-
-(* FIXME: the □ should not be needed, but removing it causes TC resolution to
-diverge. *)
 Definition msg3_pred kA m3 : iProp :=
-  □ ∃ nA nB kB,
+  ∃ nA nB kB,
     ⌜m3 = Spec.of_list [nA; nB; TKey Dec kB]⌝ ∧
     session cr_sess_name Init kA kB nA nB.
-
-Global Instance msg3_pred_persistent kA m3 :
-  Persistent (msg3_pred kA m3).
-Proof. by apply _. Qed.
-
-Lemma msg3_pred_elimG `{Decision G} (ts : list term) kA kB nA nB :
-  ts !! 0 = Some nA →
-  ts !! 1 = Some nB →
-  ts !! 2 = Some (TKey Dec kB) →
-  guarded G (msg3_pred kA (Spec.of_list ts)) -∗
-  guarded G (session cr_sess_name Init kA kB nA nB).
-Proof.
-iIntros (ts_0 ts_1 ts_2) "tsP".
-rewrite /guarded; case: decide => //= _.
-iDestruct "tsP" as (nA' nB' kA') "[%e #sess]".
-by move/Spec.of_list_inj: e ts_0 ts_1 ts_2 => -> [] -> [] -> [] ->.
-Qed.
-
-Definition cr_key_inv rl k : iProp :=
-  termT Pub (TKey Dec k) ∗
-  stermT Sec (TKey Enc k).
-Arguments cr_key_inv : simpl never.
-
-Global Instance cr_key_inv_persistent rl k :
-  Persistent (cr_key_inv rl k).
-Proof. rewrite /cr_key_inv; case: rl; apply _. Qed.
-
-Lemma cr_key_inv_pub rl k : cr_key_inv rl k -∗ termT Pub (TKey Dec k).
-Proof. by iDestruct 1 as "[??]". Qed.
-
-Definition cr_keys_inv Ks : iProp := (
-  [∗ list] rl ∈ [Init; Resp],
-  [∗ set]  k  ∈ cr_honest_proj rl Ks,
-    cr_key_inv rl k
-)%I.
-
-Lemma cr_keys_inv_elim rl k Ks :
-  k ∈ cr_honest_proj rl Ks →
-  cr_keys_inv Ks -∗
-  cr_key_inv rl k.
-Proof.
-case: rl => [] /= k_Ks; iIntros "inv"; rewrite /cr_keys_inv /=.
-- iDestruct "inv" as "[inv _]".
-  by rewrite big_sepS_forall; iApply "inv".
-- iDestruct "inv" as "(_ & inv & _)".
-  by rewrite big_sepS_forall; iApply "inv".
-Qed.
 
 Variable cr_sess_inv : role → term → term → term → term → iProp.
 
@@ -143,119 +50,139 @@ Definition cr_inv : iProp :=
   session_inv cr_sess_name (cryptoN.@"cr") cr_sess_inv.
 
 Definition cr_ctx : iProp :=
-  session_ctx cr_sess_name (cryptoN.@"cr") cr_sess_inv ∧
-  auth_ctx cr_honest_name (cryptoN.@"cr") id cr_keys_inv.
-
-Lemma cr_key_elim E rl k :
-  ↑cryptoN.@"cr" ⊆ E →
-  cr_ctx -∗
-  cr_key rl k ={E}=∗
-  ▷ cr_key_inv rl k.
-Proof.
-iIntros (?) "[_ #ctx] #key".
-iMod (auth_acc id cr_keys_inv with "[ctx key]") as "inv"; eauto.
-iDestruct "inv" as (Ks) "(%k_K & #inv & close)".
-iMod ("close" $! Ks with "[]") as "_"; first by iSplit; eauto.
-move: k_K; rewrite cr_res_of_key_included /= => k_K.
-by iIntros "!> !>"; iApply cr_keys_inv_elim; eauto.
-Qed.
-
-Lemma cr_key_elimG `{Decision G} E rl k :
-  ↑cryptoN.@"cr" ⊆ E →
-  cr_ctx -∗
-  guarded G (cr_key rl k) ={E}=∗
-  ▷ guarded G (cr_key_inv rl k).
-Proof.
-iIntros (?) "ctx key_k"; rewrite /guarded; case: decide => //= _.
-by iApply (cr_key_elim with "ctx key_k").
-Qed.
+  session_ctx cr_sess_name (cryptoN.@"cr") cr_sess_inv.
 
 Variable send recv gen : val.
 
 Ltac protocol_failure :=
   by intros; wp_pures; iApply ("Hpost" $! None).
 
-Definition initiator (skA pkA pkB nA : val) : val := λ: <>,
-  let:  "m1"   := term_of_list [nA; pkA] in
+Definition initiator : val := λ: "skA" "pkA" "pkB" "nA",
+  let:  "m1"   := term_of_list ["nA"; "pkA"] in
   send  "m1";;
-  bind: "m2"   := tdec (nroot.@"m2") pkB (recv #()) in
+  bind: "m2"   := tdec (nroot.@"m2") "pkB" (recv #()) in
   bind: "m2"   := list_of_term "m2" in
   bind: "nA'"  := "m2" !! #0 in
   bind: "nB"   := "m2" !! #1 in
   bind: "pkA'" := "m2" !! #2 in
-  if: eq_term "nA'" nA && eq_term "pkA'" pkA then
-    let:  "m3" := term_of_list [nA; "nB"; pkB] in
-    bind: "m3" := tenc (nroot.@"m3") skA "m3" in
+  if: eq_term "nA'" "nA" && eq_term "pkA'" "pkA" then
+    let:  "m3" := term_of_list ["nA"; "nB"; "pkB"] in
+    bind: "m3" := tenc (nroot.@"m3") "skA" "m3" in
     send "m3";;
     SOME "nB"
   else NONE.
 
-Definition responder (skB pkB : val) : val := λ: <>,
+Definition responder : val := λ: "skB" "pkB",
   bind: "m1"   := list_of_term (recv #()) in
   bind: "nA"   := "m1" !! #0 in
   bind: "pkA"  := "m1" !! #1 in
   bind: "kt"   := is_key "pkA" in
   if: "kt" = repr Dec then
     let:  "nB"   := gen #() in
-    bind: "m2"   := tenc (nroot.@"m2") skB (term_of_list ["nA"; "nB"; "pkA"]) in
+    bind: "m2"   := tenc (nroot.@"m2") "skB" (term_of_list ["nA"; "nB"; "pkA"]) in
     send  "m2";;
     bind: "m3"   := tdec (nroot.@"m3") "pkA" (recv #()) in
     bind: "m3"   := list_of_term "m3" in
     bind: "nA'"  := "m3" !! #0 in
     bind: "nB'"  := "m3" !! #1 in
     bind: "pkB'" := "m3" !! #2 in
-    if: eq_term "nA'" "nA" && eq_term "nB'" "nB" && eq_term "pkB'" pkB then
+    if: eq_term "nA'" "nA" && eq_term "nB'" "nB" && eq_term "pkB'" "pkB" then
       SOME ("pkA", "nA", "nB")
     else NONE
   else NONE.
+
 Implicit Types Ψ : val → iProp.
 
 Hypothesis wp_send : forall E t Ψ,
-  ▷ termT Pub t -∗
+  ▷ pterm t -∗
   Ψ #() -∗
   WP send t @ E {{ Ψ }}.
 
 Hypothesis wp_recv : forall E Ψ,
-  (∀ t, termT Pub t -∗ Ψ t) -∗
+  (∀ t, pterm t -∗ Ψ t) -∗
   WP recv #() @ E {{ Ψ }}.
 
 Hypothesis wp_gen : forall E kA kB nA Ψ,
   (∀ nB, cr_sess_inv Resp kA kB nA nB -∗
-         crypto_meta_token nB (↑cryptoN.@"cr") -∗
-         termT Pub nB -∗
+         crypto_meta_token nB (↑cryptoN.@"cr".@nB) -∗
+         pterm nB -∗
          Ψ nB) -∗
   WP gen #() @ E {{ Ψ }}.
 
-Lemma wp_initiator kA lB kB nA E Ψ :
+Lemma pterm_msg2E m2 kA kB nA nB :
+  m2 !! Z.to_nat 0 = Some nA →
+  m2 !! Z.to_nat 1 = Some nB →
+  m2 !! Z.to_nat 2 = Some (TKey Dec kA) →
+  crypto_enc (nroot.@"m2") msg2_pred -∗
+  pterm (TKey Dec kB) -∗
+  pterm (TEnc kB (Spec.tag (nroot.@"m2") (Spec.of_list m2))) -∗
+  ▷ (pterm nB ∧
+     (pterm (TKey Enc kB) ∨ session cr_sess_name Resp kA kB nA nB)).
+Proof.
+iIntros (enA enB ekA) "#enc_m2 #p_d_kB #p_m2".
+rewrite pterm_TEnc; iDestruct "p_m2" as "[[p_e_kB p_m2]|p_m2]".
+  rewrite pterm_tag pterm_of_list.
+  iPoseProof (big_sepL_lookup with "p_m2") as "p_nB"; first exact: enB.
+  iSplit => //.
+  by eauto.
+iDestruct "p_m2" as "(_ & inv & #pub)".
+iSpecialize ("pub" with "p_d_kB").
+rewrite pterm_tag pterm_of_list.
+iPoseProof (big_sepL_lookup with "pub") as "p_nB"; first exact: enB.
+iSplit => //.
+iPoseProof (enc_inv_elim with "inv enc_m2") as "{inv} #inv".
+iModIntro.
+iDestruct "inv" as (nA' nB' kA') "(%e_m2 & #sess)".
+move/Spec.of_list_inj: e_m2 enA enB ekA => -> /= [] -> [] -> [] ->.
+by eauto.
+Qed.
+
+Lemma pterm_msg3E m3 kA kB nA nB :
+  m3 !! Z.to_nat 0 = Some nA →
+  m3 !! Z.to_nat 1 = Some nB →
+  m3 !! Z.to_nat 2 = Some (TKey Dec kB) →
+  crypto_enc (nroot.@"m3") msg3_pred -∗
+  pterm (TKey Dec kA) -∗
+  pterm (TEnc kA (Spec.tag (nroot.@"m3") (Spec.of_list m3))) -∗
+  ▷ (pterm (TKey Enc kA) ∨ session cr_sess_name Init kA kB nA nB).
+Proof.
+iIntros (enA enB ekB) "#enc_m3 #p_d_ka #p_m3".
+rewrite pterm_TEnc; iDestruct "p_m3" as "[[p_e_kA p_m3]|p_m3]".
+  by eauto.
+iDestruct "p_m3" as "(_ & inv & _)".
+iPoseProof (enc_inv_elim with "inv enc_m3") as "{inv} #inv".
+iModIntro.
+iDestruct "inv" as (nA' nB' kB') "[%e_m3 inv]".
+move/Spec.of_list_inj: e_m3 enA enB ekB => -> /= [] -> [] -> [] ->.
+by eauto.
+Qed.
+
+Lemma wp_initiator kA kB nA E Ψ :
   ↑cryptoN.@"cr" ⊆ E →
   cr_ctx -∗
-  crypto_inv_meta (nroot.@"m2") msg2_pred -∗
-  crypto_inv_meta (nroot.@"m3") msg3_pred -∗
-  termT Pub nA -∗
+  crypto_enc (nroot.@"m2") msg2_pred -∗
+  crypto_enc (nroot.@"m3") msg3_pred -∗
+  pterm nA -∗
   (∀ nB, cr_sess_inv Init kA kB nA nB) -∗
-  crypto_meta_token nA (↑cryptoN.@"cr") -∗
-  cr_key Init kA -∗
-  termT Pub (TKey Dec kB) -∗
-  stermT lB (TKey Enc kB) -∗
+  crypto_meta_token nA (↑cryptoN.@"cr".@nA) -∗
+  pterm (TKey Dec kA) -∗
+  pterm (TKey Dec kB) -∗
   (∀ onB : option term,
       (if onB is Some nB then
-         termT Pub nB ∗
-         guarded (lB = Sec) (cr_sess_inv Resp kA kB nA nB)
+         pterm nB ∧
+         (pterm (TKey Enc kB) ∨ cr_sess_inv Resp kA kB nA nB)
        else True) -∗
       Ψ (repr onB)) -∗
-  WP initiator (TKey Enc kA) (TKey Dec kA) (TKey Dec kB) nA #() @ E
+  WP initiator (TKey Enc kA) (TKey Dec kA) (TKey Dec kB) nA @ E
      {{ Ψ }}.
 Proof.
 rewrite /initiator.
-iIntros (?) "#ctx #inv2 #inv3 #HnA inv_nA unreg #HkA #HkB_lo #HkB_enc Hpost".
-iMod (cr_key_elim with "ctx HkA") as "#HkA_inv" => //.
+iIntros (?) "#ctx #inv2 #inv3 #p_nA inv unreg #d_kA #d_kB Hpost".
 wp_list (_ :: _ :: []).
 wp_term_of_list.
 wp_pures; wp_bind (send _); iApply wp_send.
   iModIntro.
-  iApply termT_of_list => /=.
-  iDestruct "HkA_inv" as "(?&?)".
-  by do !iSplit.
+  by iApply pterm_of_list => /=; eauto.
 wp_pures; wp_bind (recv _); iApply wp_recv.
 iIntros (m2) "#Hm2"; wp_tdec m2; last protocol_failure.
 wp_list_of_term m2; last protocol_failure.
@@ -264,99 +191,92 @@ wp_lookup nB  enB; last protocol_failure.
 wp_lookup pkB' epkB'; last protocol_failure.
 wp_eq_term e; last protocol_failure; subst nA'.
 wp_eq_term e; last protocol_failure; subst pkB'.
-iPoseProof (termT_adec_sec_pubG
-              with "HkB_enc inv2 HkB_lo Hm2") as "{Hm2} [Hm2 #fragB]"; eauto.
-rewrite termT_of_list.
-iPoseProof (big_sepL_lookup with "Hm2") as "m2_nB"; first exact: enB.
+iPoseProof (pterm_msg2E with "[//] d_kB Hm2")
+  as "{Hm2} [p_nB sessB]" => //.
 wp_list (_ :: _ :: _ :: []); wp_term_of_list.
 wp_tenc; wp_pures.
-iPoseProof (msg2_pred_elimG with "fragB") as "{fragB} fragB"; eauto.
-iMod (session_begin with "[] [inv_nA] [unreg]") as "[#sessA close]".
-- by eauto.
-- by iDestruct "ctx" as "[??]".
-- by iApply "inv_nA".
-- by eauto.
-iAssert (|={E}=> ▷ guarded (lB = Sec) (cr_sess_inv Resp kA kB nA nB))%I
+iSpecialize ("inv" $! nB).
+iMod (session_begin with "[] inv [unreg]") as "[#sessA close]"; eauto.
+iAssert (|={E}=> ▷ (pterm (TKey Enc kB) ∨ cr_sess_inv Resp kA kB nA nB))%I
     with "[close]" as ">inv".
-  rewrite /guarded; case: decide => [_|//].
-  by iApply "close".
+  iDestruct "sessB" as "[?|sessB]"; eauto.
+  by iMod ("close" with "sessB") as "close"; eauto.
 wp_bind (send _); iApply wp_send.
-  iModIntro.
-  iDestruct "HkA_inv" as "(?&?)".
-  iApply termT_aenc_sec_pub => //.
-  - by iApply stermT_termT.
-  - by rewrite termT_of_list /=; do !iSplit.
-  - iIntros "!> !>"; by iExists _, _, _; iSplit.
+  iModIntro; iApply pterm_TEncIS; eauto.
+  - iPoseProof (pterm_sterm with "d_kA") as "?".
+    by rewrite !sterm_TKey.
+  - iModIntro.
+    iExists _, _, _; iSplit => //.
+    by rewrite sterm_of_list /= -!pterm_sterm; eauto.
+  - iIntros "!> _".
+    by rewrite pterm_of_list /=; eauto.
 wp_pures; iApply ("Hpost" $! (Some nB)).
 by iFrame.
 Qed.
 
-Lemma wp_responder kA kB E Ψ :
+Lemma wp_responder kB E Ψ :
   ↑cryptoN.@"cr" ⊆ E →
   cr_ctx -∗
-  crypto_inv_meta (nroot.@"m2") msg2_pred -∗
-  crypto_inv_meta (nroot.@"m3") msg3_pred -∗
-  cr_key Init kA -∗
-  cr_key Resp kB -∗
+  crypto_enc (nroot.@"m2") msg2_pred -∗
+  crypto_enc (nroot.@"m3") msg3_pred -∗
+  pterm (TKey Dec kB) -∗
   (∀ ot : option (term * term * term),
       (if ot is Some (pkA, nA, nB) then
-         ∃ kA',
-           ⌜pkA = TKey Dec kA'⌝ ∗
-           termT Pub nA ∗
-           termT Pub nB ∗
-           termT Pub (TKey Dec kA') ∗
-           guarded (kA' = kA) (cr_sess_inv Init kA kB nA nB)
+         ∃ kA,
+           ⌜pkA = TKey Dec kA⌝ ∗
+           pterm pkA ∧
+           pterm nA ∧
+           pterm nB ∧
+           (pterm (TKey Enc kA) ∨ cr_sess_inv Init kA kB nA nB)
        else True) -∗
        Ψ (repr ot)) -∗
-  WP responder (TKey Enc kB) (TKey Dec kB) #() @ E {{ Ψ }}.
+  WP responder (TKey Enc kB) (TKey Dec kB) @ E {{ Ψ }}.
 Proof.
-iIntros (?) "#ctx #inv2 #inv3 #HkA #HkB Hpost".
-iMod (cr_key_elim with "ctx HkA") as "# (?&?)" => //.
-iMod (cr_key_elim with "ctx HkB") as "# (?&?)" => //.
+iIntros (?) "#ctx #enc2 #enc3 #HkB Hpost".
 rewrite /responder; wp_pures.
 wp_bind (recv _); iApply wp_recv; iIntros (m1) "#Hm1".
 wp_list_of_term m1; last protocol_failure.
 wp_lookup nA enA; last protocol_failure.
 wp_lookup pkA epkA; last protocol_failure.
-rewrite termT_of_list.
+rewrite pterm_of_list.
 iPoseProof (big_sepL_lookup with "Hm1") as "HnA"; first exact: enA.
 iPoseProof (big_sepL_lookup with "Hm1") as "HpkA"; first exact: epkA.
 iClear "Hm1".
-wp_is_key_eq kt kA' et; last protocol_failure; subst pkA.
+wp_is_key_eq kt kA et; last protocol_failure; subst pkA.
 wp_pures.
 case: (bool_decide_reflect (_ = repr_key_type Dec)); last protocol_failure.
 case: kt epkA=> // epkA _.
 wp_pures; wp_bind (gen _); iApply wp_gen; iIntros (nB) "inv token #HnB".
 iMod (session_begin with "[] inv [token]") as "[#sessB close]".
 - by eauto.
-- by iDestruct "ctx" as "[??]".
+- by eauto.
 - by eauto.
 wp_list (_ :: _ :: _ :: []); wp_term_of_list.
 wp_tenc; wp_pures; wp_bind (send _); iApply wp_send.
   iModIntro.
-  iApply termT_aenc_sec_pub.
-  - by iApply stermT_termT.
+  iApply pterm_TEncIS.
+  - iPoseProof (pterm_sterm with "HkB") as "?".
+    by rewrite !sterm_TKey.
   - by eauto.
-  - by rewrite termT_of_list /=; do !iSplit.
-  - iModIntro; iExists _, _, _; eauto.
+  - iIntros "!>". by iExists _, _, _; eauto.
+  - by rewrite sterm_of_list /= -!pterm_sterm; eauto.
+  - iIntros "!> _".
+    by rewrite pterm_of_list /=; eauto.
 wp_pures; wp_bind (recv _); iApply wp_recv; iIntros (m3) "#Hm3".
 wp_tdec m3; last protocol_failure.
 wp_list_of_term m3; last protocol_failure.
-iAssert (▷^2 guarded (kA' = kA) (msg3_pred kA (Spec.of_list m3)))%I
-    as "{Hm3} Hm3".
-  rewrite /guarded; case: decide => [e|//]; subst kA'.
-  by iPoseProof (termT_adec_sec_pub (nroot.@"m3") _ kA with "[//] [//] [//] Hm3")
-    as "[_ #sessA]".
 wp_lookup nA' enA'; last protocol_failure.
 wp_lookup nB' enB'; last protocol_failure.
 wp_lookup pkB' epkB'; last protocol_failure.
 wp_eq_term e; last protocol_failure; subst nA'.
 wp_eq_term e; last protocol_failure; subst nB'.
 wp_eq_term e; last protocol_failure; subst pkB'.
-iPoseProof (msg3_pred_elimG with "Hm3") as "sessA" => //.
-iAssert (|={E}=> ▷ (guarded (kA' = kA) (cr_sess_inv Init kA kB nA nB)))%I
+iPoseProof (pterm_msg3E with "[//] HpkA Hm3") as "{Hm3} Hm3"; eauto.
+wp_if.
+iAssert (|={E}=> ▷ (pterm (TKey Enc kA) ∨ cr_sess_inv Init kA kB nA nB))%I
     with "[close]" as ">inv".
-  rewrite /guarded; case: decide => [->|//]; by iApply "close".
+  iDestruct "Hm3" as "[Hm3 | Hm3]"; eauto.
+  iMod ("close" with "Hm3") as "close". by eauto.
 wp_pures; iApply ("Hpost" $! (Some (_, _, _))).
 by iExists _; do ![iSplit=> //].
 Qed.
